Phi_Semantics/PhiSem_Aggregate_Tuple.thy
@@ -92,8 +92,13 @@ lemma Tuple_Field_expn[\<phi>expns]:
   \<open>p \<in> (x \<Ztypecolon> \<lbrace> T \<rbrace>) \<longleftrightarrow> (\<exists>v. p = V_tup.mk [v] \<and> v \<in> (x \<Ztypecolon> T))\<close>
   unfolding Tuple_Field_def \<phi>Type_def by simp
 
-lemma Tuple_Field_inhabited[elim!,\<phi>inhabitance_rule]:
+lemma Tuple_Field_inhabited[elim!]:
   \<open>Inhabited (x \<Ztypecolon> \<lbrace> T \<rbrace>) \<Longrightarrow> (Inhabited (x \<Ztypecolon> T) \<Longrightarrow> C) \<Longrightarrow> C\<close>
+  unfolding Inhabited_def by (simp add: \<phi>expns)
+
+lemma [\<phi>inhabitance_rule 1000]:
+  \<open> Inhabited (x \<Ztypecolon> T) \<longrightarrow> C
+\<Longrightarrow> Inhabited (x \<Ztypecolon> \<lbrace> T \<rbrace>) \<longrightarrow> C \<close>
   unfolding Inhabited_def by (simp add: \<phi>expns)
 
 lemma Empty_Tuple_reduce[simp]:
